Foundation/Propositional/Formula.lean
@@ -214,37 +214,37 @@ instance : Encodable (Formula α) where
 end Encodable
 
 
-def letterless : Formula α → Prop
+def Letterless : Formula α → Prop
   | .atom _ => False
   | ⊥ => True
-  | φ ➝ ψ => (φ.letterless) ∧ (ψ.letterless)
-  | φ ⋏ ψ => (φ.letterless) ∧ (ψ.letterless)
-  | φ ⋎ ψ => (φ.letterless) ∧ (ψ.letterless)
+  | φ ➝ ψ => (φ.Letterless) ∧ (ψ.Letterless)
+  | φ ⋏ ψ => (φ.Letterless) ∧ (ψ.Letterless)
+  | φ ⋎ ψ => (φ.Letterless) ∧ (ψ.Letterless)
 
-namespace letterless
+namespace Letterless
 
 variable {φ ψ : Formula α}
 
-@[simp] lemma not_atom : ¬(letterless (atom p)) := by simp [letterless]
+@[simp] lemma not_atom : ¬(Letterless (atom p)) := by simp [Letterless]
 
-@[simp] lemma def_bot : (⊥ : Formula α).letterless := by simp [letterless]
+@[simp] lemma def_bot : (⊥ : Formula α).Letterless := by simp [Letterless]
 
-@[simp] lemma def_top : (⊤ : Formula α).letterless := by simp [letterless]
+@[simp] lemma def_top : (⊤ : Formula α).Letterless := by simp [Letterless]
 
 
-lemma def_imp : (φ ➝ ψ).letterless → φ.letterless ∧ ψ.letterless := by simp [letterless]
-lemma def_imp₁ : (φ ➝ ψ).letterless → φ.letterless := λ h => def_imp h |>.1
-lemma def_imp₂ : (φ ➝ ψ).letterless → ψ.letterless := λ h => def_imp h |>.2
+lemma def_imp : (φ ➝ ψ).Letterless → φ.Letterless ∧ ψ.Letterless := by simp [Letterless]
+@[grind] lemma def_imp₁ : (φ ➝ ψ).Letterless → φ.Letterless := λ h => def_imp h |>.1
+@[grind] lemma def_imp₂ : (φ ➝ ψ).Letterless → ψ.Letterless := λ h => def_imp h |>.2
 
-lemma def_and : (φ ⋏ ψ).letterless → φ.letterless ∧ ψ.letterless := by simp [letterless]
-lemma def_and₁ : (φ ⋏ ψ).letterless → φ.letterless := λ h => def_and h |>.1
-lemma def_and₂ : (φ ⋏ ψ).letterless → ψ.letterless := λ h => def_and h |>.2
+lemma def_and : (φ ⋏ ψ).Letterless → φ.Letterless ∧ ψ.Letterless := by simp [Letterless]
+@[grind] lemma def_and₁ : (φ ⋏ ψ).Letterless → φ.Letterless := λ h => def_and h |>.1
+@[grind] lemma def_and₂ : (φ ⋏ ψ).Letterless → ψ.Letterless := λ h => def_and h |>.2
 
-lemma def_or : (φ ⋎ ψ).letterless → φ.letterless ∧ ψ.letterless := by simp [letterless]
-lemma def_or₁ : (φ ⋎ ψ).letterless → φ.letterless := λ h => def_or h |>.1
-lemma def_or₂ : (φ ⋎ ψ).letterless → ψ.letterless := λ h => def_or h |>.2
+lemma def_or : (φ ⋎ ψ).Letterless → φ.Letterless ∧ ψ.Letterless := by simp [Letterless]
+@[grind] lemma def_or₁ : (φ ⋎ ψ).Letterless → φ.Letterless := λ h => def_or h |>.1
+@[grind] lemma def_or₂ : (φ ⋎ ψ).Letterless → ψ.Letterless := λ h => def_or h |>.2
 
-end letterless
+end Letterless
 
 end Formula
 
@@ -451,10 +451,10 @@ infixr:80 " ∘ " => Substitution.comp
 lemma Formula.subst_comp {s₁ s₂ : Substitution α} {φ : Formula α} : φ⟦s₁ ∘ s₂⟧ = φ⟦s₁⟧⟦s₂⟧ := by
   induction φ <;> simp_all [Substitution.comp];
 
-def ZeroSubstitution (α) := { s : Substitution α // ∀ {a : α}, ((.atom a)⟦s⟧).letterless }
+def ZeroSubstitution (α) := { s : Substitution α // ∀ {a : α}, ((.atom a)⟦s⟧).Letterless }
 
-lemma Formula.letterless_zeroSubst {φ : Formula α} {s : ZeroSubstitution α} : (φ⟦s.1⟧).letterless := by
-  induction φ <;> simp [Formula.letterless, *];
+lemma Formula.Letterless_zeroSubst {φ : Formula α} {s : ZeroSubstitution α} : (φ⟦s.1⟧).Letterless := by
+  induction φ <;> simp [Formula.Letterless, *];
   case hatom => exact s.2;
 
 
