Foundation/ProvabilityLogic/Classification/Trace.lean
@@ -1,152 +1,33 @@
 import Foundation.ProvabilityLogic.Classification.LetterlessTrace
 import Foundation.Modal.Boxdot.GL_S
 import Foundation.Modal.Logic.SumQuasiNormal
-
-
-namespace Set
-
-variable {α : Type*} {s t : Set α}
-
-abbrev Cofinite (s : Set α) := sᶜ.Finite
-
-abbrev Coinfinite (s : Set α) := sᶜ.Infinite
-
-lemma Cofinite.subset (h : s ⊆ t) : s.Cofinite → t.Cofinite := by
-  intro h;
-  apply Set.Finite.subset (s := sᶜ) h;
-  tauto_set;
-
-lemma Coinfinite.subset (h : t ⊆ s) : s.Coinfinite → t.Coinfinite := by
-  contrapose!;
-  simpa using Set.Cofinite.subset h;
-
-@[grind] lemma univ_cofinite : (Set.univ (α := α)).Cofinite := by simp [Set.Cofinite];
-
-@[grind]
-lemma iff_cofinite_not_coinfinite : s.Cofinite ↔ ¬s.Coinfinite := by
-  dsimp [Set.Cofinite, Set.Coinfinite];
-  simp;
-
-end Set
+import Foundation.Modal.Logic.D.Basic
 
 
 namespace LO
-
-
-namespace Semantics
-
-variable {M : Type*} {F : Type*} [LogicalConnective F] [Semantics F M] [Tarski M] {𝓜 : M} {α}
-
-@[simp] lemma realize_list_conj' {l : List α} {ι : α → F} : 𝓜 ⊧ l.conj' ι ↔ ∀ i ∈ l, 𝓜 ⊧ ι i := by simp [List.conj']
-
-@[simp] lemma realize_list_disj' {l : List α} {ι : α → F} : 𝓜 ⊧ l.disj' ι ↔ ∃ i ∈ l, 𝓜 ⊧ ι i := by simp [List.disj']
-
-@[simp] lemma realize_finset_conj' {s : Finset α} {ι : α → F} : 𝓜 ⊧ s.conj' ι ↔ ∀ i ∈ s, 𝓜 ⊧ ι i := by simp [Finset.conj']
-
-@[simp] lemma realize_finset_disj' {s : Finset α} {ι : α → F} : 𝓜 ⊧ s.disj' ι ↔ ∃ i ∈ s, 𝓜 ⊧ ι i := by simp [Finset.disj']
-
-end Semantics
-
-
-namespace Entailment
-
-variable {F : Type*} [LogicalConnective F]
-         {S : Type*} [Entailment F S]
-         {𝓢 : S} [Entailment.Minimal 𝓢]
-
-lemma FConj'_iff_forall_provable [DecidableEq F] {s : Finset α} {ι : α → F} : (𝓢 ⊢! ⩕ i ∈ s, ι i) ↔ (∀ i ∈ s, 𝓢 ⊢! ι i) := by
-  have : 𝓢 ⊢! ⋀(s.toList.map ι) ↔ ∀ i ∈ s, 𝓢 ⊢! ι i := by simpa using Conj₂!_iff_forall_provable (Γ := s.toList.map ι);
-  apply Iff.trans ?_ this;
-  simp [Finset.conj', List.conj'];
-
-end Entailment
-
-
 
 namespace Modal
 
 variable {φ ψ : Formula ℕ}
 
 open Kripke
+open Formula.Kripke
 
-namespace Kripke.Frame
 
-variable {F : Frame} {r x y : F} [Fintype F] [F.IsTree r]
+namespace Formula
 
-lemma eq_finHeight_root : Frame.World.finHeight x = F.finHeight ↔ x = r := by
-  constructor;
-  . rintro h;
-    contrapose! h;
-    apply Nat.ne_of_lt;
-    apply Frame.World.finHeight_lt_whole_finHeight;
-    apply F.root_genaretes'!;
-    assumption;
-  . tauto;
+def trace (φ : Formula ℕ) : Set ℕ := { n | ∃ M : Kripke.Model, ∃ r, ∃ _ : M.IsTree r, ∃ _ : Fintype M, (M.height = n ∧ ¬r ⊧ φ) }
 
-lemma terminal_rel_finHeight (h : x ≺^[World.finHeight x] y) : ∀ z, ¬y ≺ z := by
-  intro z Ryz;
-  suffices World.finHeight x + 1 ≤ World.finHeight x by omega;
-  exact le_finHeight_iff_relItr.mpr ⟨z, HRel.Iterate.forward.mpr ⟨y, h, Ryz⟩⟩;
+lemma iff_mem_trace {n : ℕ} : n ∈ φ.trace ↔ ∃ M : Kripke.Model, ∃ r : M, ∃ _ : M.IsTree r, ∃ _ : Fintype M, M.height = n ∧ ¬r ⊧ φ := by
+  simp [Formula.trace];
 
-lemma extendRoot.eq_original_finHeight : Frame.World.finHeight (x : F.extendRoot 1) = Frame.World.finHeight x := by
-  apply finHeight_eq_iff_relItr.mpr;
-  constructor;
-  . obtain ⟨y, Rxy⟩ := exists_terminal (i := x);
-    use y;
-    apply extendRoot.embed_rel_iterate_embed_iff_rel.mpr;
-    exact Rxy;
-  . rintro (_ | y) Rxy (_ | z);
-    . simp;
-    . -- TODO: extract no loop lemma (x ≺^[n] i cannot happen where x is original and i is new elements by extension)
-      exfalso;
-      have : extendRoot.root ≺ (x : F.extendRoot 1) := Frame.root_genaretes'! (F := F.extendRoot 1) x (by simp);
-      have : (x : F.extendRoot 1) ≺ x :=
-        HRel.Iterate.unwrap_of_trans_of_pos (by omega) $
-        HRel.Iterate.comp (m := 1) |>.mp ⟨_, Rxy, by simpa⟩;
-      exact Frame.irrefl _ this;
-    . apply Frame.asymm;
-      exact Frame.root_genaretes'! (F := F.extendRoot 1) y (by simp);
-    . have := terminal_rel_finHeight $ extendRoot.embed_rel_iterate_embed_iff_rel.mp Rxy;
-      exact extendRoot.embed_rel_embed_iff_rel.not.mpr $ this z;
-
-lemma extendRoot.eq_original_finHeight_root : Frame.World.finHeight (r : F.extendRoot 1) = F.finHeight := eq_original_finHeight
+lemma satisfies_of_not_mem_trace : n ∉ φ.trace ↔ (∀ M : Kripke.Model, ∀ r : M, [M.IsTree r] → [Fintype M] → M.height = n → r ⊧ φ) := by
+  simp [Formula.trace];
 
 @[grind]
-lemma extendRoot.iff_eq_finHeight_eq_original_root {x : F.extendRoot 1} : Frame.World.finHeight x = F.finHeight ↔ x = r := by
-  constructor;
-  . rcases x with (a | x);
-    . intro h;
-      have := h ▸ finHeight₁ (F := F);
-      simp [Frame.finHeight] at this;
-    . intro h;
-      suffices x = r by simp [this];
-      apply Frame.eq_finHeight_root.mp;
-      exact h ▸ Frame.extendRoot.eq_original_finHeight.symm;
-  . rintro rfl;
-    exact eq_original_finHeight_root;
-
-open Classical in
-noncomputable instance [h : Fintype F] : Fintype (F↾x) := by apply Subtype.fintype;
-
-instance [F.IsTree r] : (F↾x).IsTree ⟨x, by tauto⟩ := by constructor;
-
-axiom pointGenerate.eq_original_finHeight (hxy : y = x ∨ x ≺^+ y) : Frame.World.finHeight (F := F↾x) (⟨y, hxy⟩) = Frame.World.finHeight y
-
-end Kripke.Frame
-
-
-def Formula.gTrace (φ : Formula ℕ) : Set ℕ := { n | ∃ M : Kripke.Model, ∃ r, ∃ _ : M.IsTree r, ∃ _ : Fintype M, (M.finHeight = n ∧ ¬r ⊧ φ) }
-
-lemma iff_mem_gTrace {n : ℕ} : n ∈ φ.gTrace ↔ ∃ M : Kripke.Model, ∃ r : M, ∃ _ : M.IsTree r, ∃ _ : Fintype M, M.finHeight = n ∧ ¬r ⊧ φ := by
-  simp [Formula.gTrace];
-
-lemma satisfies_of_not_mem_gTrace : n ∉ φ.gTrace ↔ (∀ M : Kripke.Model, ∀ r : M, [M.IsTree r] → [Fintype M] → M.finHeight = n → r ⊧ φ) := by
-  simp [Formula.gTrace];
-
-@[grind]
-lemma Formula.eq_gTrace_trace_of_letterless {φ : Formula ℕ} (φ_letterless : φ.letterless) : φ.gTrace = φ.trace := by
+lemma eq_trace_trace_of_letterless {φ : Formula ℕ} (φ_letterless : φ.Letterless) : φ.trace = φ.letterlessTrace := by
   ext n;
-  apply Iff.trans ?_ (Kripke.spectrum_TFAE φ_letterless (n := n) |>.out 1 0 |>.not);
+  apply Iff.trans ?_ (Kripke.letterlessSpectrum_TFAE φ_letterless (n := n) |>.out 1 0 |>.not);
   constructor;
   . rintro ⟨M, r, _, M_fintype, rfl, h⟩;
     push_neg;
@@ -154,58 +35,63 @@ lemma Formula.eq_gTrace_trace_of_letterless {φ : Formula ℕ} (φ_letterless : 
     . assumption;
     . rfl;
     . assumption;
-  . dsimp [Formula.gTrace];
+  . dsimp [Formula.trace];
     contrapose!;
     rintro h M r _ _ x rfl;
     apply Model.pointGenerate.modal_equivalent' x ⟨x, by tauto⟩ |>.mp;
     apply h;
-    apply Frame.pointGenerate.eq_original_finHeight;
+    apply Frame.pointGenerate.eq_original_height;
 
 open Formula.Kripke
 
-@[simp, grind] lemma Formula.gTrace_bot : (⊥ : Formula ℕ).gTrace = Set.univ := by simp [Formula.eq_gTrace_trace_of_letterless];
-@[simp, grind] lemma Formula.gTrace_top : (⊤ : Formula ℕ).gTrace = ∅ := by simp [Formula.eq_gTrace_trace_of_letterless];
+@[simp, grind] lemma trace_bot : (⊥ : Formula ℕ).trace = Set.univ := by simp [Formula.eq_trace_trace_of_letterless];
+@[simp, grind] lemma trace_top : (⊤ : Formula ℕ).trace = ∅ := by simp [Formula.eq_trace_trace_of_letterless];
 
-lemma Formula.gTrace_and : (φ ⋏ ψ).gTrace = φ.gTrace ∪ ψ.gTrace := by
+lemma trace_and : (φ ⋏ ψ).trace = φ.trace ∪ ψ.trace := by
   ext n;
   calc
-    _ ↔ ∃ M : Kripke.Model, ∃ r : M, ∃ _ : M.IsTree r, ∃ _ : Fintype M, M.finHeight = n ∧ (¬r ⊧ φ ∨ ¬r ⊧ ψ) := by simp [gTrace, -not_and, not_and_or]
+    _ ↔ ∃ M : Kripke.Model, ∃ r : M, ∃ _ : M.IsTree r, ∃ _ : Fintype M, M.height = n ∧ (¬r ⊧ φ ∨ ¬r ⊧ ψ) := by simp [trace, -not_and, not_and_or]
     _ ↔
-      (∃ M : Kripke.Model, ∃ r : M, ∃ _ : M.IsTree r, ∃ _ : Fintype M, M.finHeight = n ∧ ¬r ⊧ φ) ∨
-      (∃ M : Kripke.Model, ∃ r : M, ∃ _ : M.IsTree r, ∃ _ : Fintype M, M.finHeight = n ∧ ¬r ⊧ ψ) := by
+      (∃ M : Kripke.Model, ∃ r : M, ∃ _ : M.IsTree r, ∃ _ : Fintype M, M.height = n ∧ ¬r ⊧ φ) ∨
+      (∃ M : Kripke.Model, ∃ r : M, ∃ _ : M.IsTree r, ∃ _ : Fintype M, M.height = n ∧ ¬r ⊧ ψ) := by
       constructor;
       . rintro ⟨M, r, _, _, _, (h | h)⟩;
         . left; tauto;
         . right; tauto;
       . rintro (⟨M, r, _, _, _, _⟩ | ⟨M, r, _, _, _, _⟩) <;>
         . refine ⟨M, r, by assumption, by assumption, by tauto⟩;
-    _ ↔ _ := by simp [Formula.gTrace];
+    _ ↔ _ := by simp [Formula.trace];
 
-lemma Formula.gTrace_lconj₂ {s : List (Formula ℕ)} : (s.conj₂).gTrace = ⋃ φ ∈ s, φ.gTrace := by
+lemma trace_lconj₂ {s : List (Formula ℕ)} : (s.conj₂).trace = ⋃ φ ∈ s, φ.trace := by
   induction s using List.induction_with_singleton with
-  | hcons φ s hs ih => simp [List.conj₂_cons_nonempty hs, Formula.gTrace_and, ih];
+  | hcons φ s hs ih => simp [List.conj₂_cons_nonempty hs, Formula.trace_and, ih];
   | _ => simp [List.conj₂];
 
-lemma Formula.gTrace_fconj {s : Finset (Formula ℕ)} : s.conj.gTrace = ⋃ φ ∈ s, φ.gTrace := by simp [Finset.conj, Formula.gTrace_lconj₂];
+lemma trace_fconj {s : Finset (Formula ℕ)} : s.conj.trace = ⋃ φ ∈ s, φ.trace := by simp [Finset.conj, Formula.trace_lconj₂];
 
-lemma subset_gTrace_of_provable_imp_GL (h : Modal.GL ⊢! φ ➝ ψ) : ψ.gTrace ⊆ φ.gTrace := by
+lemma subset_trace_of_provable_imp_GL (h : Modal.GL ⊢! φ ➝ ψ) : ψ.trace ⊆ φ.trace := by
   intro n hn;
-  obtain ⟨M, r, _, _, rfl, h₁⟩ := iff_mem_gTrace.mp hn;
-  apply iff_mem_gTrace.mpr;
+  obtain ⟨M, r, _, _, rfl, h₁⟩ := iff_mem_trace.mp hn;
+  apply iff_mem_trace.mpr;
   refine ⟨M, r, by assumption, by assumption, by rfl, ?_⟩;
   contrapose! h₁;
   have : M.IsFiniteTree r := {}
   apply GL.Kripke.iff_provable_satisfies_FiniteTransitiveTree.mp h;
   assumption;
 
-abbrev FormulaSet.gTrace (X : FormulaSet ℕ) : Set ℕ := ⋃ φ ∈ X, φ.gTrace
+end Formula
 
-@[simp] lemma FormulaSet.gTrace_empty : (∅ : FormulaSet ℕ).gTrace = ∅ := by simp [FormulaSet.gTrace];
 
-lemma eq_FormulaSet_gTrace_finset_conj {X : Finset (Formula ℕ)} : X.conj.gTrace = FormulaSet.gTrace X.toSet := by simp [FormulaSet.gTrace, Formula.gTrace_fconj];
+namespace FormulaSet
 
-lemma FormulaSet.subset_gTrace_of_subset {X Y : FormulaSet ℕ} (h : X ⊆ Y) : X.gTrace ⊆ Y.gTrace := by
-  simp only [gTrace, Set.iUnion_subset_iff];
+abbrev trace (X : FormulaSet ℕ) : Set ℕ := ⋃ φ ∈ X, φ.trace
+
+@[simp] lemma trace_empty : (∅ : FormulaSet ℕ).trace = ∅ := by simp [FormulaSet.trace];
+
+lemma eq_FormulaSet_trace_finset_conj {X : Finset (Formula ℕ)} : X.conj.trace = FormulaSet.trace X.toSet := by simp [FormulaSet.trace, Formula.trace_fconj];
+
+lemma subset_trace_of_subset {X Y : FormulaSet ℕ} (h : X ⊆ Y) : X.trace ⊆ Y.trace := by
+  simp only [trace, Set.iUnion_subset_iff];
   intro φ hφ i hi;
   simp only [Set.mem_iUnion, exists_prop];
   use φ;
@@ -213,18 +99,21 @@ lemma FormulaSet.subset_gTrace_of_subset {X Y : FormulaSet ℕ} (h : X ⊆ Y) : 
   . apply h; assumption;
   . assumption;
 
-abbrev Logic.trace (L : Logic ℕ) : Set ℕ := FormulaSet.gTrace L
+end FormulaSet
 
-lemma GL.eq_trace_ext {X : FormulaSet ℕ} (hX : ∀ ξ ∈ X, ∀ s : Substitution _, ξ⟦s⟧ ∈ X) : (Modal.GL.sumQuasiNormal X).trace = X.gTrace := by
+
+abbrev Logic.trace (L : Logic ℕ) : Set ℕ := FormulaSet.trace L
+
+lemma GL.eq_trace_ext {X : FormulaSet ℕ} (hX : ∀ ξ ∈ X, ∀ s : Substitution _, ξ⟦s⟧ ∈ X) : (Modal.GL.sumQuasiNormal X).trace = X.trace := by
   ext n;
   constructor;
-  . suffices (∃ φ, Modal.GL.sumQuasiNormal X ⊢! φ ∧ n ∈ φ.gTrace) → (n ∈ X.gTrace) by simpa [Logic.trace];
+  . suffices (∃ φ, Modal.GL.sumQuasiNormal X ⊢! φ ∧ n ∈ φ.trace) → (n ∈ X.trace) by simpa [Logic.trace, Logic.iff_provable];
     rintro ⟨φ, hφ₁, hφ₂⟩;
     obtain ⟨Y, hY₁, hY₂⟩ := Logic.sumQuasiNormal.iff_provable_finite_provable hX |>.mp hφ₁;
-    apply FormulaSet.subset_gTrace_of_subset hY₁;
-    apply eq_FormulaSet_gTrace_finset_conj ▸ subset_gTrace_of_provable_imp_GL hY₂;
+    apply FormulaSet.subset_trace_of_subset hY₁;
+    apply FormulaSet.eq_FormulaSet_trace_finset_conj ▸ Formula.subset_trace_of_provable_imp_GL hY₂;
     assumption;
-  . suffices (∃ φ ∈ X, n ∈ φ.gTrace) → (∃ φ, Modal.GL.sumQuasiNormal X ⊢! φ ∧ n ∈ φ.gTrace) by simpa [Logic.trace];
+  . suffices (∃ φ ∈ X, n ∈ φ.trace) → (∃ φ, Modal.GL.sumQuasiNormal X ⊢! φ ∧ n ∈ φ.trace) by simpa [Logic.trace, Logic.iff_provable];
     rintro ⟨φ, hφ₁, hφ₂⟩;
     use φ;
     constructor;
@@ -232,15 +121,15 @@ lemma GL.eq_trace_ext {X : FormulaSet ℕ} (hX : ∀ ξ ∈ X, ∀ s : Substitut
       simpa [Logic.iff_provable];
     . assumption;
 
-lemma GL.unprovable_of_exists_trace (φ_letterless : φ.letterless) : (∃ n, n ∈ φ.trace) → Modal.GL ⊬ φ := by
+lemma GL.unprovable_of_exists_trace (φ_letterless : φ.Letterless) : (∃ n, n ∈ φ.letterlessTrace) → Modal.GL ⊬ φ := by
   contrapose!;
   intro h;
-  have := Modal.iff_GL_provable_spectrum_Univ φ_letterless |>.mp (by simpa using h);
-  simp_all [Formula.trace];
+  have := Modal.iff_GL_provable_letterlessSpectrum_Univ φ_letterless |>.mp (by simpa using h);
+  simp_all [Formula.letterlessTrace];
 
 @[simp]
-lemma TBBMinus_trace (hβ : βᶜ.Finite) : (∼⩕ n ∈ hβ.toFinset, TBB n).trace = β := by
-  simp [Formula.trace, TBBMinus_spectrum']
+lemma TBBMinus_trace (hβ : β.Cofinite) : (∼⩕ n ∈ hβ.toFinset, TBB n).letterlessTrace = β := by
+  simp [Formula.letterlessTrace, TBBMinus_letterlessSpectrum']
 
 @[simp]
 lemma GL.eq_trace_emptyset : Modal.GL.trace = ∅ := by
@@ -250,12 +139,12 @@ lemma GL.eq_trace_emptyset : Modal.GL.trace = ∅ := by
 @[simp]
 lemma GLα.eq_trace {α : Set ℕ} : (Modal.GLα α).trace = α := by
   apply Eq.trans $ GL.eq_trace_ext $ by grind;
-  simp [FormulaSet.gTrace, Formula.eq_gTrace_trace_of_letterless];
+  simp [FormulaSet.trace, Formula.eq_trace_trace_of_letterless];
 
 @[simp]
-lemma GLβMinus.eq_trace {β : Set ℕ} (hβ : βᶜ.Finite := by grind) : (Modal.GLβMinus β).trace = β := by
+lemma GLβMinus.eq_trace {β : Set ℕ} (hβ : β.Cofinite := by grind) : (Modal.GLβMinus β).trace = β := by
   apply Eq.trans $ GL.eq_trace_ext $ by grind;
-  simp [FormulaSet.gTrace, Formula.eq_gTrace_trace_of_letterless];
+  simp [FormulaSet.trace, Formula.eq_trace_trace_of_letterless];
 
 @[simp, grind] lemma S.provable_TBB {n : ℕ} : Modal.S ⊢! TBB n := by simp [TBB]
 
@@ -270,39 +159,23 @@ lemma subset_GLα_S : Modal.GLα α ⊆ Modal.S := by
   | mdp ihφψ ihφ => exact ihφψ ⨀ ihφ;
   | subst ihφ => exact Logic.subst! _ ihφ;
 
-@[grind]
-lemma Logic.weakerThan_of_subset {L₁ L₂ : Logic α} (h : L₁ ⊆ L₂) : L₁ ⪯ L₂ := by
-  constructor;
-  simpa [Entailment.theory];
-
-@[grind]
-lemma Logic.strictWeakerThan_of_ssubset {L₁ L₂ : Logic α} (h : L₁ ⊂ L₂) : L₁ ⪱ L₂ := by
-  simp_all [Entailment.strictlyWeakerThan_iff, Set.ssubset_iff_exists];
-  aesop;
-
 instance : Modal.GLα α ⪯ Modal.S := by grind
-
-@[simp, grind]
-lemma Logic.subset_of_weakerThan {L₁ L₂ : Logic α} [L₁ ⪯ L₂] : L₁ ⊆ L₂ := by
-  intro φ;
-  suffices L₁ ⊢! φ → L₂ ⊢! φ by grind;
-  exact Entailment.WeakerThan.pbl;
 
 @[simp]
 lemma S.eq_trace : Modal.S.trace = Set.univ := by
-  suffices ∀ (x : ℕ), ∃ i ∈ Modal.S, x ∈ i.gTrace by simpa [Set.eq_univ_iff_forall]
+  suffices ∀ (x : ℕ), ∃ i ∈ Modal.S, x ∈ i.trace by simpa [Set.eq_univ_iff_forall]
   intro n;
   use (TBB n);
   constructor;
   . grind;
-  . simp [Formula.eq_gTrace_trace_of_letterless];
+  . simp [Formula.eq_trace_trace_of_letterless];
 
 variable {L : Logic ℕ} {φ : Formula ℕ}
 
 
-lemma subset_of_provable (h : L ⊢! φ) : φ.gTrace ⊆ L.trace := by
+lemma subset_of_provable (h : L ⊢! φ) : φ.trace ⊆ L.trace := by
   intro n h;
-  suffices ∃ i ∈ L, n ∈ i.gTrace by simpa [Logic.trace, FormulaSet.gTrace];
+  suffices ∃ i ∈ L, n ∈ i.trace by simpa [Logic.trace, FormulaSet.trace];
   use φ;
   grind;
 
@@ -380,22 +253,22 @@ instance isTree [M.IsTree r] (hra : r ≠ a) : (M.boneLengthening a k).IsTree r 
       tauto;
 
 @[simp]
-axiom height [M.IsTree r] [Fintype M] (hra : r ≠ a) :
+axiom eq_height [M.IsTree r] [Fintype M] (hra : r ≠ a) :
   have : (M.boneLengthening a k).IsTree r := isTree hra;
-  (M.boneLengthening a k).finHeight = M.finHeight + k
+  (M.boneLengthening a k).height = M.height + k
   /-
   := by
   intro _;
-  apply finHeight_eq_iff_relItr.mpr;
+  apply height_eq_iff_relItr.mpr;
   constructor;
-  . obtain ⟨t, Rrt⟩ := Kripke.exists_terminal (F := M.boneLengthening a k |>.toFrame) r;
+  . obtain ⟨t, Rrt⟩ := Kripke.exists_rank_terminal (F := M.boneLengthening a k |>.toFrame) r;
     use t;
     induction k with
     | zero =>
       sorry;
     | succ k ih =>
-      suffices (r : M.boneLengthening a (k + 1)) ≺^[(M.finHeight + k) + 1] t by
-        rwa [(show M.finHeight + (k + 1) = (M.finHeight + k) + 1 by omega)];
+      suffices (r : M.boneLengthening a (k + 1)) ≺^[(M.rank + k) + 1] t by
+        rwa [(show M.rank + (k + 1) = (M.rank + k) + 1 by omega)];
       dsimp [Frame.RelItr', HRel.Iterate]
       sorry;
   . intro t Rrt x;
@@ -461,63 +334,52 @@ end Kripke
 axiom GL.formalized_validates_axiomT_set_in_irrefl_trans_chain : Modal.GL ⊢! ∼□^[(φ.rflSubformula.card + 1)]⊥ ➝ ◇φ.rflSubformula.conj
 
 @[grind]
-lemma Formula.gTrace.finite_or_cofinite : φ.gTrace.Finite ∨ φ.gTrace.Cofinite := by
-  suffices φ.gTrace.Infinite → φ.gTrace.Cofinite by tauto;
+lemma Formula.trace.finite_or_cofinite : φ.trace.Finite ∨ φ.trace.Cofinite := by
+  suffices φ.trace.Infinite → φ.trace.Cofinite by tauto;
   intro tr_infinite;
 
-  obtain ⟨m, hm₁, hm₂⟩ : ∃ m, m ∈ φ.gTrace ∧ φ.rflSubformula.card < m  := Set.infinite_iff_exists_gt.mp tr_infinite _;
+  obtain ⟨m, hm₁, hm₂⟩ : ∃ m, m ∈ φ.trace ∧ φ.rflSubformula.card < m  := Set.infinite_iff_exists_gt.mp tr_infinite _;
 
-  obtain ⟨M, r,_, _, rfl, hr⟩ := iff_mem_gTrace.mp hm₁;
+  obtain ⟨M, r,_, _, rfl, hr⟩ := iff_mem_trace.mp hm₁;
   have : M.IsFiniteTree r := {}
 
-  have H₁ : r ⊧ ∼□^[(φ.rflSubformula.card + 1)]⊥ := finHeight_lt_iff_satisfies_boxbot (i := r) (n := φ.rflSubformula.card + 1) |>.not.mp $ by
-    rw [←Frame.finHeight];
+  have H₁ : r ⊧ ∼□^[(φ.rflSubformula.card + 1)]⊥ := height_lt_iff_satisfies_boxbot (i := r) (n := φ.rflSubformula.card + 1) |>.not.mp $ by
+    rw [←Frame.height];
     omega;
   have H₂ : r ⊧ ∼□^[(φ.rflSubformula.card + 1)]⊥ ➝ ◇φ.rflSubformula.conj := GL.Kripke.iff_provable_satisfies_FiniteTransitiveTree.mp (GL.formalized_validates_axiomT_set_in_irrefl_trans_chain) M r;
   obtain ⟨a, Rrx, hx⟩ := Satisfies.dia_def.mp $ H₂ H₁;
   replace Rrx : r ≠ a := by rintro rfl; apply M.irrefl _ Rrx;
 
-  have : {k | k ≥ M.finHeight} ⊆ φ.gTrace := by
+  have : {k | k ≥ M.height} ⊆ φ.trace := by
     intro k hmk;
     obtain ⟨k, rfl⟩ := Nat.exists_eq_add_of_le hmk;
-    apply iff_mem_gTrace.mpr;
+    apply iff_mem_trace.mpr;
     refine ⟨M.boneLengthening a k, r, ?_, ?_, ?_, ?_⟩;
     . apply Model.boneLengthening.isTree Rrx;
     . infer_instance;
-    . apply Model.boneLengthening.height Rrx;
+    . apply Model.boneLengthening.eq_height Rrx;
     . exact Model.boneLengthening.mainlemma₂ hx (by grind) r |>.not.mp hr;
   apply Set.Cofinite.subset this;
-  apply Set.Finite.subset (s := Finset.range M.finHeight);
+  apply Set.Finite.subset (s := Finset.range M.height);
   . apply Finset.finite_toSet;
   . intro i;
     simp;
 
 @[grind]
-lemma Formula.gTrace.finite_of_coinfinite (h_ci : φ.gTrace.Coinfinite) : φ.gTrace.Finite := by
-  rcases Formula.gTrace.finite_or_cofinite (φ := φ) with h | h_cf;
+lemma Formula.trace.finite_of_coinfinite (h_ci : φ.trace.Coinfinite) : φ.trace.Finite := by
+  rcases Formula.trace.finite_or_cofinite (φ := φ) with h | h_cf;
   . assumption;
   . exfalso;
     apply h_ci;
     exact h_cf;
 
-@[simp]
-lemma TBB_injective : Function.Injective TBB := by
-  rintro i j;
-  suffices □^[i]⊥ = □^[j]⊥ → i = j by simpa;
-  wlog hij : i < j;
-  . rcases (show i = j ∨ i > j by omega) with h | h
-    . tauto;
-    . have := @this j i; grind;
-  obtain ⟨k, rfl⟩ := Nat.exists_eq_add_of_lt hij;
-  simp [show ((i + k) + 1) = i + (k + 1) by omega, ←(Box.add (n := i) (m := (k + 1)))];
-
 lemma subset_GLα_of_trace_coinfinite (hL : L.trace.Coinfinite) : L ⊆ Modal.GLα L.trace := by
   intro φ hφ;
   apply Modal.Logic.iff_provable.mp;
 
-  have : φ.gTrace ⊆ L.trace := subset_of_provable (by grind);
-  have : φ.gTrace.Finite := by
-    have : φ.gTrace.Coinfinite := Set.Coinfinite.subset this hL
+  have : φ.trace ⊆ L.trace := subset_of_provable (by grind);
+  have : φ.trace.Finite := by
+    have : φ.trace.Coinfinite := Set.Coinfinite.subset this hL
     grind
   let Tφ := this.toFinset;
 
@@ -527,40 +389,22 @@ lemma subset_GLα_of_trace_coinfinite (hL : L.trace.Coinfinite) : L ⊆ Modal.GL
   . apply GL.Kripke.tree_completeness_TFAE.out 3 0 |>.mp;
     intro M r _ hr;
     have : Fintype M.World := Fintype.ofFinite _;
-    apply satisfies_of_not_mem_gTrace (n := M.finHeight) |>.mp;
-    . replace hr : ∀ n ∈ φ.gTrace, M.finHeight ≠ n := by
+    apply Formula.satisfies_of_not_mem_trace (n := M.height) |>.mp;
+    . replace hr : ∀ n ∈ φ.trace, M.height ≠ n := by
         intro n h;
-        apply iff_satisfies_TBB_ne_finHeight.mp;
+        apply iff_satisfies_TBB_ne_rank.mp;
         apply Satisfies.fconj_def.mp hr _;
-        suffices ∃ m ∈ φ.gTrace, □^[m]⊥ = □^[n]⊥ by simpa [Tφ];
+        suffices ∃ m ∈ φ.trace, □^[m]⊥ = □^[n]⊥ by simpa [Tφ];
         use n;
       by_contra hC;
       apply hr _ hC rfl;
     . rfl;
 
-
-namespace Formula.Kripke.Satisfies
-
-variable {M : Kripke.Model} {w : M} {X : Finset α} {ι : α → Formula ℕ} {φ ψ : Formula ℕ}
-
-lemma fconj'_def : w ⊧ (⩕ i ∈ X, ι i) ↔ ∀ i ∈ X, w ⊧ ι i := by simp;
-
-lemma not_fconj'_def : ¬(w ⊧ (⩕ i ∈ X, ι i)) ↔ ∃ i ∈ X, ¬(w ⊧ ι i) := by simp;
-
-lemma fdisj'_def : w ⊧ (⩖ i ∈ X, ι i) ↔ ∃ i ∈ X, w ⊧ ι i := by simp;
-
-lemma not_fdisj'_def : ¬(w ⊧ (⩖ i ∈ X, ι i)) ↔ ∀ i ∈ X, ¬(w ⊧ ι i) := by simp;
-
-lemma not_and_def : ¬(w ⊧ φ ⋏ ψ) ↔ ¬(w ⊧ φ) ∨ ¬(w ⊧ ψ) := by simp [-not_and, not_and_or];
-
-end Formula.Kripke.Satisfies
-
-
 lemma subset_GLβMinus_of_trace_cofinite (hL : L.trace.Cofinite) : L ⊆ Modal.GLβMinus L.trace := by
   intro φ hφ;
   apply Modal.Logic.iff_provable.mp;
 
-  have : φ.gTrace ⊆ L.trace := subset_of_provable (by grind);
+  have : φ.trace ⊆ L.trace := subset_of_provable (by grind);
 
   let Tφ := hL.toFinset;
 
@@ -570,18 +414,18 @@ lemma subset_GLβMinus_of_trace_cofinite (hL : L.trace.Cofinite) : L ⊆ Modal.G
   . apply GL.Kripke.tree_completeness_TFAE.out 3 0 |>.mp;
     intro M r _ hr;
     have : Fintype M.World := Fintype.ofFinite _;
-    apply satisfies_of_not_mem_gTrace (n := M.finHeight) |>.mp;
-    . replace hr : ∀ (n : ℕ), ∀ x ∈ L, n ∈ x.gTrace → ¬M.finHeight = n := by
+    apply Formula.satisfies_of_not_mem_trace (n := M.height) |>.mp;
+    . replace hr : ∀ (n : ℕ), ∀ x ∈ L, n ∈ x.trace → ¬M.height = n := by
         rintro n ξ hξ₁ hξ₂ rfl;
         obtain ⟨m, hm₁, hm₂⟩ : ∃ m, m ∈ Tφ ∧ ¬r ⊧ TBB m := Satisfies.not_fconj'_def.mp $ Satisfies.not_def.mp $ by
           simpa only [Finset.conj_singleton] using hr;
-        replace hm₁ : ∀ i ∈ L, m ∉ i.gTrace := by simpa [Tφ] using hm₁;
-        replace hm₂ : M.finHeight = m := by simpa using iff_satisfies_TBB_ne_finHeight.not.mp hm₂;
+        replace hm₁ : ∀ i ∈ L, m ∉ i.trace := by simpa [Tφ] using hm₁;
+        replace hm₂ : M.height = m := by simpa using iff_satisfies_TBB_ne_rank.not.mp hm₂;
         apply hm₁ ξ;
         . assumption;
         . grind;
       by_contra hC;
-      apply hr M.finHeight φ hφ hC rfl;
+      apply hr M.height φ hφ hC rfl;
     . rfl;
 
 protected abbrev GLαOmega := Modal.GLα Set.univ
@@ -598,10 +442,10 @@ lemma eq_GLβMinusOmega : Modal.GLβMinus Set.univ = Set.univ := by
   . suffices Modal.GL ⊢! ∼⊤ ➝ φ by simpa;
     cl_prover;
 
-protected abbrev D_inter_GLβMinus (β : Set ℕ) (hβ : βᶜ.Finite := by grind) := Modal.D ∩ Modal.GLβMinus β
+protected abbrev D_inter_GLβMinus (β : Set ℕ) (hβ : β.Cofinite := by grind) := Modal.D ∩ Modal.GLβMinus β
 @[simp] lemma eq_D_inter_GLβMinusOmega : Modal.D_inter_GLβMinus Set.univ = Modal.D := by simp
 
-protected abbrev S_inter_GLβMinus (β : Set ℕ) (hβ : βᶜ.Finite := by grind) := Modal.S ∩ Modal.GLβMinus β
+protected abbrev S_inter_GLβMinus (β : Set ℕ) (hβ : β.Cofinite := by grind) := Modal.S ∩ Modal.GLβMinus β
 @[simp] lemma eq_S_inter_GLβMinusOmega : Modal.S_inter_GLβMinus Set.univ = Modal.S := by simp
 
 end Modal
@@ -630,44 +474,44 @@ lemma provable_TBB_of_mem_trace {n : ℕ} (h : n ∈ (T.ProvabilityLogic U).trac
   have : M₀.IsFiniteTree r₀ := {};
   let S : SolovaySentences T.standardProvability M₀.toFrame r₀ := SolovaySentences.standard T M₀.toFrame;
 
-  have : M₀ ⊧ A ➝ (Modal.TBB M.finHeight) := by
+  have : M₀ ⊧ A ➝ (Modal.TBB M.height) := by
     rintro x hA;
-    rcases Nat.lt_trichotomy (Frame.World.finHeight x) M.finHeight with h | h | h;
+    rcases Nat.lt_trichotomy (Frame.rank x) M.height with h | h | h;
     . intro _;
-      exact finHeight_lt_iff_satisfies_boxbot.mp h;
+      exact height_lt_iff_satisfies_boxbot.mp h;
     . exfalso;
       suffices x = r by
         apply h₂;
         apply Kripke.Model.extendRoot.modal_equivalence_original_world.mpr;
         rwa [this] at hA;
-      apply Kripke.Frame.extendRoot.iff_eq_finHeight_eq_original_root.mp h;
-    . apply iff_satisfies_mem_finHeight_spectrum (by grind) |>.mpr;
+      apply Kripke.Frame.extendRoot.iff_eq_height_eq_original_root.mp h;
+    . apply iff_satisfies_mem_rank_letterlessSpectrum (by grind) |>.mpr;
       simp;
       omega;
-  have : ∀ i : M₀.World, 𝗜𝚺₁ ⊢! S i ➝ S.realization (A ➝ (Modal.TBB M.finHeight)) := by
+  have : ∀ i : M₀.World, 𝗜𝚺₁ ⊢! S i ➝ S.realization (A ➝ (Modal.TBB M.height)) := by
     rintro (a | i);
-    . suffices 𝗜𝚺₁ ⊢! S r₀ ➝ S.realization (TBB M.finHeight) by
+    . suffices 𝗜𝚺₁ ⊢! S r₀ ➝ S.realization (TBB M.height) by
         dsimp [Realization.interpret];
         rw [(show Sum.inl a = r₀ by simp [r₀])];
         cl_prover [this]
-      have : 𝗜𝚺₁ ⊢! S r₀ ➝ ∼(T.standardProvability) (S.realization (□^[M.finHeight]⊥)) := C!_trans (S.SC2 r₀ r Rr₀) $ contra! $
+      have : 𝗜𝚺₁ ⊢! S r₀ ➝ ∼(T.standardProvability) (S.realization (□^[M.height]⊥)) := C!_trans (S.SC2 r₀ r Rr₀) $ contra! $
         T.standardProvability.prov_distribute_imply' $
         CN!_of_CN!_right $
         S.mainlemma_neg Rr₀ $
-        finHeight_lt_iff_satisfies_boxbot.not.mp $ by simp [Frame.extendRoot.eq_original_finHeight_root]
+        height_lt_iff_satisfies_boxbot.not.mp $ by simp [Frame.extendRoot.eq_original_height_root]
       apply C!_trans this
       simp [Realization.interpret.def_boxItr]
     . apply S.mainlemma Rr₀;
       apply this;
-  have : 𝗜𝚺₁ ⊢! (⩖ j, S j) ➝ S.realization (A ➝ (Modal.TBB M.finHeight)) := left_Udisj!_intro _ this
-  have : 𝗜𝚺₁ ⊢! S.realization (A ➝ (Modal.TBB M.finHeight)) := by cl_prover [this, S.SC4];
+  have : 𝗜𝚺₁ ⊢! (⩖ j, S j) ➝ S.realization (A ➝ (Modal.TBB M.height)) := left_Udisj!_intro _ this
+  have : 𝗜𝚺₁ ⊢! S.realization (A ➝ (Modal.TBB M.height)) := by cl_prover [this, S.SC4];
 
-  have : U ⊢! S.realization (Modal.TBB M.finHeight) := by
-    have : U ⊢! S.realization A ➝ S.realization (Modal.TBB M.finHeight) := WeakerThan.pbl this;
+  have : U ⊢! S.realization (Modal.TBB M.height) := by
+    have : U ⊢! S.realization A ➝ S.realization (Modal.TBB M.height) := WeakerThan.pbl this;
     cl_prover [this, hA₁ S.realization];
   apply ProvabilityLogic.provable_iff.mpr;
   intro g;
-  simpa [Realization.letterless_interpret (A := Modal.TBB _) (by grind)] using this;
+  grind;
 
 theorem eq_provablityLogic_GLα_of_coinfinite_trace (h : (T.ProvabilityLogic U).trace.Coinfinite) : T.ProvabilityLogic U = Modal.GLα (T.ProvabilityLogic U).trace := by
   apply Set.Subset.antisymm;
@@ -708,7 +552,7 @@ lemma provable_TBBMinus_of_mem_trace (h : ¬(T.ProvabilityLogic U) ⊆ Modal.S) 
   let r₀ : M₀.World := Model.extendRoot.root;
   have : Fintype M₀.World := Fintype.ofFinite _
 
-  let R := Set.Finite.inter_of_left (s := (Finset.range M₁.finHeight)) (t := (T.ProvabilityLogic U).trace) (Finset.finite_toSet _) |>.toFinset;
+  let R := Set.Finite.inter_of_left (s := (Finset.range M₁.height)) (t := (T.ProvabilityLogic U).trace) (Finset.finite_toSet _) |>.toFinset;
 
   let B := A ⋏ ⩕ i ∈ R, TBB i;
   have hB : T.ProvabilityLogic U ⊢! B := by
@@ -743,18 +587,17 @@ lemma provable_TBBMinus_of_mem_trace (h : ¬(T.ProvabilityLogic U) ⊆ Modal.S) 
       . intro h;
         apply Satisfies.not_def.mpr;
         apply Satisfies.not_fconj'_def.mpr;
-        use Frame.World.finHeight (i : M₀);
+        use Frame.rank (i : M₀);
         constructor;
         . by_contra hC;
-          apply iff_satisfies_TBB_ne_finHeight (w := (i : M₀)) (n := Frame.World.finHeight (i : M₀)) |>.mp;
+          apply iff_satisfies_TBB_ne_rank (w := (i : M₀)) (n := Frame.rank (i : M₀)) |>.mp;
           . apply Satisfies.fconj'_def.mp $ Satisfies.and_def.mp h |>.2;
-            suffices Frame.World.finHeight (i : M₀) < M₁.finHeight ∧ Frame.World.finHeight (i : M₀) ∈ (T.ProvabilityLogic U).trace by
-              simpa [R];
+            suffices Frame.rank (i : M₀) < M₁.height ∧ Frame.rank (i : M₀) ∈ (T.ProvabilityLogic U).trace by simpa [R];
             constructor;
-            . suffices Frame.World.finHeight i < M₁.finHeight by calc
-                _ = Frame.World.finHeight (i : M₁) := by convert Frame.extendRoot.eq_original_finHeight
-                _ < _                              := this;
-              apply Frame.World.finHeight_lt_whole_finHeight;
+            . suffices Frame.rank i < M₁.height by calc
+                _ = Frame.rank (i : M₁) := by convert Frame.extendRoot.eq_original_height
+                _ < _                   := this;
+              apply Frame.rank_lt_whole_height;
               apply M₁.root_genaretes'!;
               rintro rfl;
               apply Satisfies.not_imp_def.mp hM |>.2;
@@ -762,7 +605,7 @@ lemma provable_TBBMinus_of_mem_trace (h : ¬(T.ProvabilityLogic U) ⊆ Modal.S) 
               exact Satisfies.and_def.mp h |>.1;
             . simpa using hC;
           . rfl;
-        . apply iff_satisfies_TBB_ne_finHeight.not.mpr;
+        . apply iff_satisfies_TBB_ne_rank.not.mpr;
           simp;
 
   replace H₁ : U ⊢! S.realization B ➝ S.realization (∼⩕ n ∈ (cofinite_of_not_subset_S h).toFinset, TBB n) := WeakerThan.pbl H₁;
@@ -771,8 +614,7 @@ lemma provable_TBBMinus_of_mem_trace (h : ¬(T.ProvabilityLogic U) ⊆ Modal.S) 
 
   apply ProvabilityLogic.provable_iff.mpr;
   intro g;
-
-  rwa [Realization.letterless_interpret (f₁ := S.realization) (f₂ := g) (by grind)] at H;
+  grind;
 
 /-- Artemov & Beklemishev. Lemma 49 -/
 theorem eq_provabilityLogic_GLβMinus_of_not_subset_S (h : ¬(T.ProvabilityLogic U) ⊆ Modal.S) : T.ProvabilityLogic U = Modal.GLβMinus (T.ProvabilityLogic U).trace := by
