Foundation/Modal/Hilbert/WithHenkin/Basic.lean
@@ -107,8 +107,9 @@ section
 
 abbrev logic (H : Hilbert.WithHenkin α) : Logic α := Entailment.theory H
 
-@[simp high]
-lemma iff_logic_provable_provable : H.logic ⊢! φ ↔ H ⊢! φ := by simp [logic, Entailment.theory, Set.mem_setOf_eq];
+@[grind]
+lemma iff_logic_provable_provable : H.logic ⊢! φ ↔ H ⊢! φ := by
+  simp [Logic.iff_provable, logic, Entailment.theory, Set.mem_setOf_eq];
 
 instance [H₁ ⪯ H₂] : H₁.logic ⪯ H₂.logic := by
   apply weakerThan_iff.mpr;
