Foundation/Propositional/Logic/PostComplete.lean
@@ -3,14 +3,6 @@ import Foundation.Propositional.Kripke.Logic.Cl
 import Foundation.Propositional.ClassicalSemantics.Hilbert
 import Foundation.Propositional.ClassicalSemantics.ZeroSubst
 
-lemma Set.ssubset_of_subset_ne {α : Type*} {s t : Set α} (h : s ⊆ t) (hne : s ≠ t) : s ⊂ t := by
-  constructor;
-  . assumption;
-  . revert hne;
-    contrapose!;
-    intro _;
-    apply Set.eq_of_subset_of_subset <;> assumption;
-
 namespace LO.Propositional
 
 namespace Logic
@@ -31,7 +23,7 @@ theorem Cl.post_complete : ¬∃ L : Logic _, Entailment.Consistent L ∧ Nonemp
   have h₁ : L ⊢! ∼(φ⟦(vfSubst v).1⟧) := hL $ by
     apply iff_isTautology.mpr;
     apply neg_isTautology_of_not_isTautology_of_letterless;
-    . apply Formula.letterless_zeroSubst;
+    . apply Formula.Letterless_zeroSubst;
     . apply isTautology_vfSubst.not.mp hv;
   have h₂ : L ⊢! φ⟦(vfSubst v).1⟧ := L.subst! _ hφ₂;
   exact h₁ ⨀ h₂;
