Foundation/Vorspiel/Finset/Supplemental.lean
@@ -2,9 +2,9 @@ import Mathlib.Data.Finset.Insert
 
 namespace Finset
 
-variable {α : Type*} [DecidableEq α] {a b : α} {s : Finset α}
+variable {α : Type*} {a b : α} {s : Finset α}
 
-lemma doubleton_subset : ({a, b} : Finset α) ⊆ s ↔ a ∈ s ∧ b ∈ s := by
+lemma doubleton_subset [DecidableEq α] : ({a, b} : Finset α) ⊆ s ↔ a ∈ s ∧ b ∈ s := by
   constructor;
   . intro h;
     have ⟨ha, hb⟩ := Finset.insert_subset_iff.mp h;
@@ -14,5 +14,17 @@ lemma doubleton_subset : ({a, b} : Finset α) ⊆ s ↔ a ∈ s ∧ b ∈ s := b
     constructor;
     . assumption;
     . simpa;
+
+/-
+  Thanks to @plp127
+
+  https://leanprover.zulipchat.com/#narrow/channel/217875-Is-there-code-for-X.3F/topic/ascending.2Fdecending.20lemmata.20related.20.60Set.60.20and.20.60Finset.60/near/539367015
+-/
+lemma no_ssubset_descending_chain  {f : ℕ → Finset α} : ¬(∀ i, ∃ j > i, f j ⊂ f i) := by
+  intro h
+  have n := 0
+  induction hf : f n using WellFoundedLT.fix generalizing n with subst hf | _ _ ih
+  obtain ⟨m, -, hy⟩ := h n
+  exact ih (f m) hy m rfl
 
 end Finset
