Foundation/Vorspiel/Set/Cofinite.lean
@@ -1,0 +1,45 @@
+import Mathlib.Data.Finset.Insert
+import Mathlib.Data.Set.Insert
+import Mathlib.Data.Set.Countable
+import Mathlib.Tactic.TautoSet
+
+namespace Set
+
+variable {α : Type*} {s t : Set α} {a b : α}
+
+abbrev Cofinite (s : Set α) := sᶜ.Finite
+
+abbrev Coinfinite (s : Set α) := sᶜ.Infinite
+
+@[grind]
+lemma iff_cofinite_not_coinfinite : s.Cofinite ↔ ¬s.Coinfinite := by simp;
+
+@[simp] lemma iff_cofinite_comp_finite : s.Cofinite ↔ sᶜ.Finite := by simp [Cofinite];
+
+@[simp] lemma iff_coinfinite_comp_infinite : s.Coinfinite ↔ sᶜ.Infinite := by simp [Coinfinite];
+
+@[grind]
+lemma Cofinite.subset (h : s ⊆ t) : s.Cofinite → t.Cofinite := by
+  intro h;
+  apply Set.Finite.subset (s := sᶜ) h;
+  tauto_set;
+
+@[grind]
+lemma Coinfinite.subset (h : t ⊆ s) : s.Coinfinite → t.Coinfinite := by
+  contrapose!;
+  suffices t.Cofinite → s.Cofinite by grind;
+  grind;
+
+@[simp, grind] lemma univ_cofinite : (Set.univ (α := α)).Cofinite := by simp [Set.Cofinite];
+
+@[grind]
+lemma cofinite_union_left (hs : s.Cofinite) : (s ∪ t).Cofinite := by
+  simp only [Cofinite, compl_union];
+  apply Set.Finite.inter_of_left;
+  assumption;
+
+@[grind]
+lemma cofinite_union_right (ht : t.Cofinite) : (s ∪ t).Cofinite := by
+  exact (show (t ∪ s) = (s ∪ t) by tauto_set) ▸ cofinite_union_left ht;
+
+end Set
